ind proc

Constellation/ProcessesWithAtomic.lean
@@ -23,34 +23,57 @@ abbrev Holds := Finset Var
 
 abbrev Pending := List Process
 
-inductive Exec: EndoRel (Pending × Holds) where
-  | halt P H:
-      Process.halt ∈ P →
-      Exec (P, H) (P.erase Process.halt, H)
+mutual
+  inductive Exec: EndoRel (Pending × Holds) where
+    | halt P H:
+        Process.halt ∈ P →
+        Exec (P, H) (P.erase Process.halt, H)
 
-  | add P H v:
-      Process.add v ∈ P →
-      Exec (P, H) (P.erase (Process.add v), insert v H)
+    | add P H v:
+        Process.add v ∈ P →
+        Exec (P, H) (P.erase (Process.add v), insert v H)
 
-  | rem P H v:
-      Process.rem v ∈ P →
-      Exec (P, H) (P.erase (Process.rem v), H.erase v)
+    | rem P H v:
+        Process.rem v ∈ P →
+        Exec (P, H) (P.erase (Process.rem v), H.erase v)
 
-  | par P H p1 p2:
-      p1.par p2 ∈ P →
-      Exec (P, H) (p1 :: p2 :: P.erase (p1.par p2), H)
+    | par P H p1 p2:
+        p1.par p2 ∈ P →
+        Exec (P, H) (p1 :: p2 :: P.erase (p1.par p2), H)
 
-  | seq P H H' p1 p2:
-      p1.seq p2 ∈ P →
-      Exec⊹ ([p1], H) ([], H') →
-      Exec  (P, H) (p2 :: P.erase (p1.seq p2), H')
+    | seq P H H' p1 p2:
+        p1.seq p2 ∈ P →
+        Completes ([p1], H) ([], H') →
+        Exec      (P, H) (p2 :: P.erase (p1.seq p2), H')
 
-  | ite_t P H v t e:
-      Process.ite v t e ∈ P →
-      v ∈ H →
-      Exec (P, H) (t :: P.erase (Process.ite v t e), H)
+    | ite_t P H v t e:
+        Process.ite v t e ∈ P →
+        v ∈ H →
+        Exec (P, H) (t :: P.erase (Process.ite v t e), H)
 
-  | ite_e P H v t e:
-      Process.ite v t e ∈ P →
-      v ∉ H →
-      Exec (P, H) (e :: P.erase (Process.ite v t e), H)
+    | ite_e P H v t e:
+        Process.ite v t e ∈ P →
+        v ∉ H →
+        Exec (P, H) (e :: P.erase (Process.ite v t e), H)
+
+  inductive Completes: EndoRel (Pending × Holds) where
+    | intro P H H':
+        Exec⋆     (P, H) ([], H') →
+        Completes (P, H) ([], H')
+end
+
+theorem completes_empty:
+  ∀ P H P' H',
+    Completes (P,H) (P',H') →
+    P'=[]
+:= by
+  intro _ _ _ _ h
+  cases h
+  rfl
+
+theorem empty_completes (H: Holds):
+  ∃ E, Completes ([], H) E
+:= by
+  exists ([], H)
+  constructor
+  constructor
